Prove that pure expressions run purely.
If we manage to prove a total correctness result for a pure expression, by
adequacy, we can construct a sequence of pure steps that leads to a final result
that satisfies the post condition.

cryptis/lib.v
@@ -540,6 +540,133 @@ case: y => /=; first by split.
 by move=> ?; rewrite elem_of_singleton; split; congruence.
 Qed.
 
+Fixpoint pure_expr e : bool :=
+  match e with
+  | Val v => pure_val v
+  | Var _ => true
+  | Rec f x e => pure_expr e
+  | App e1 e2 => pure_expr e1 && pure_expr e2
+  | UnOp _ e => pure_expr e
+  | BinOp _ e1 e2 => pure_expr e1 && pure_expr e2
+  | If e1 e2 e3 => pure_expr e1 && pure_expr e2 && pure_expr e3
+  | Pair e1 e2 => pure_expr e1 && pure_expr e2
+  | Fst e | Snd e => pure_expr e
+  | InjL e | InjR e => pure_expr e
+  | Case e1 e2 e3 => pure_expr e1 && pure_expr e2 && pure_expr e3
+  | Fork _ => false
+  | AllocN _ _ => false
+  | Free _ => false
+  | Load _ => false
+  | Store _ _ => false
+  | CmpXchg _ _ _ => false
+  | Xchg _ _ => false
+  | FAA _ _ => false
+  | NewProph => false
+  | Resolve _ _ _ => false
+  end
+
+with pure_val v : bool :=
+  match v with
+  | LitV _ => true
+  | RecV _ _ e => pure_expr e
+  | PairV v1 v2 => pure_val v1 && pure_val v2
+  | InjLV v | InjRV v => pure_val v
+  end.
+
+Definition pure_item (a : ectx_item) : bool :=
+  match a with
+  | AppLCtx v => pure_val v
+  | AppRCtx e => pure_expr e
+  | UnOpCtx _ => true
+  | BinOpLCtx _ v => pure_val v
+  | BinOpRCtx _ e => pure_expr e
+  | IfCtx e1 e2 => pure_expr e1 && pure_expr e2
+  | PairLCtx v => pure_val v
+  | PairRCtx e => pure_expr e
+  | FstCtx | SndCtx | InjLCtx | InjRCtx => true
+  | CaseCtx e1 e2 => pure_expr e1 && pure_expr e2
+  | _ => false
+  end.
+
+Definition pure_ctx K : bool := forallb pure_item K.
+
+Section WithSsrBool.
+
+Import ssreflect ssrbool.
+
+Lemma pure_expr_fill_item a (e : expr) : pure_expr (fill_item a e) = pure_item a && pure_expr e.
+Proof.
+case: a=> //=; try by move=> *; rewrite andbC.
+- by move=> ??; rewrite [RHS]andbC andbA.
+- by move=> ??; rewrite [RHS]andbC andbA.
+Qed.
+
+Lemma pure_expr_fill K (e : expr) : pure_expr (fill K e) = pure_ctx K && pure_expr e.
+Proof.
+elim: K=> //= a K IH in e *.
+by rewrite IH pure_expr_fill_item andbA [pure_ctx K && _]andbC.
+Qed.
+
+Lemma subst_pure x v e : pure_val v → pure_expr e → pure_expr (subst x v e).
+Proof.
+move=> /is_trueP pure_v /is_trueP pure_e; apply/is_trueP.
+elim: e pure_e => //=.
+- by move=> ? _; case: decide.
+- by move=> ??? IH pure_e; case: decide => // _; eauto.
+- by move=> e1 IH1 e2 IH2 /andP [??]; rewrite IH1 // ?IH2.
+- by move=> _ e1 IH1 e2 IH2 /andP [??]; rewrite IH1 // ?IH2.
+- by move=> e1 IH1 e2 IH2 e3 IH3 /andP [/andP[??] ?]; rewrite IH1 // ?IH2 // ?IH3.
+- by move=> e1 IH1 e2 IH2 /andP [??]; rewrite IH1 // ?IH2.
+- by move=> e1 IH1 e2 IH2 e3 IH3 /andP [/andP[??] ?]; rewrite IH1 // ?IH2 // ?IH3.
+Qed.
+
+Lemma subst'_pure x v e : pure_val v → pure_expr e → pure_expr (subst' x v e).
+Proof. case: x => //= x. exact: subst_pure. Qed.
+
+Lemma pure_exprP (e1 : expr) σ1 κs e2 σ2 efs :
+  prim_step e1 σ1 κs e2 σ2 efs →
+  pure_expr e1 →
+  pure_expr e2.
+Proof.
+move=> [K {}e1 {}e2 -> ->] Hstep; rewrite !pure_expr_fill.
+case/andb_True=> /is_trueP -> //= pure_e1.
+case: e1 σ1 κs e2 σ2 efs / Hstep pure_e1 => //=.
+- move=> f x e1 v2 e' σ -> /= /andb_True [pure_e1 pure_e2].
+  apply: subst'_pure => //.
+  by apply: subst'_pure => //.
+- case=> [] [] //=.
+  + by case=> // [l|b] ? ? [<-].
+  + by case=> // n ? ? [<-].
+- move=> op v1 v2 v' σ; rewrite /bin_op_eval.
+  case: (decide (op = EqOp)) => [_|be].
+  + by case: decide=> // _ [<-] _; eauto.
+  + case: v1 v2 => //=; case=> //= [n1|b1|l1].
+    * case=> //; case=> //= n2.
+      by case: op => //= in be *; case=> <-; eauto.
+    * case=> //; case=> //= b2.
+      by case: op => //= in be *; case=> <-; eauto.
+    * by case=> // l2; case: op=> //= in be *; case: l2 => //= ? [<-]; eauto.
+- by move=> ??? /andb_True [??]; eauto.
+- by move=> ??? /andb_True [??]; eauto.
+- by move=> ??? /andb_True [??]; eauto.
+- by move=> ??? /andb_True [??]; eauto.
+- by move=> ???? /is_trueP/andP [/andP[-> ->]_]; eauto.
+- by move=> ???? /is_trueP/andP [/andP[-> _]->]; eauto.
+Qed.
+
+Lemma pure_expr_pure_step (e₁ : expr) σ₁ κs e₂ σ₂ efs :
+  prim_step e₁ σ₁ κs e₂ σ₂ efs →
+  pure_expr e₁ →
+  pure_step e₁ e₂.
+Proof.
+move=> [K {}e₁ {}e₂ -> ->] Hstep; rewrite !pure_expr_fill.
+case/andb_True=> //= pure_K pure_e₁.
+apply: pure_step_ctx => //=; apply: nsteps_once_inv.
+case: e₁ σ₁ κs e₂ σ₂ efs / Hstep pure_e₁ => //= *; subst; exact: pure_exec.
+Qed.
+
+End WithSsrBool.
+
 Fixpoint free_vars e : gset string :=
   match e with
   | Val _ => ∅
