cryptis/lib/gen_adequacy.v
@@ -10,11 +10,12 @@ Context `{!irisGS_gen HasNoLc Λ Σ}.
 Implicit Types (e : expr Λ) (v : val Λ) (es : list (expr Λ)).
 Implicit Types (Φ : val Λ → iProp Σ).
 
+Definition thread_step (p1 p2 : expr Λ * state Λ) : Prop :=
+  ∃ efs, prim_step p1.1 p1.2 [] p2.1 p2.2 efs.
+
 Definition runs_until e Φ : iProp Σ :=
-  ∀ es1 es2 σ ns ks nt, state_interp σ ns ks nt ={⊤}=∗ ∃ v es' σ' ns' ks' nt',
-    ⌜rtc erased_step
-      (es1 ++ e :: es2, σ)
-      (es1 ++ (of_val v) :: es2 ++ es', σ')⌝ ∗
+  ∀ σ ns ks nt, state_interp σ ns ks nt ={⊤}=∗ ∃ v σ' ns' ks' nt',
+    ⌜rtc thread_step (e, σ) (of_val v, σ')⌝ ∗
     state_interp σ' ns' ks' nt' ∗
     Φ v.
 
@@ -28,24 +29,23 @@ Proof.
   iRevert (HE). iRevert (e E Φ) "He". iApply twp_ind.
   { solve_proper. }
   iIntros "!>" (e E Φ); iIntros "IH" (->).
-  rewrite /twp_pre. iIntros (es1 es2 σ ns ks nt) "state".
+  rewrite /twp_pre. iIntros (σ ns ks nt) "state".
   case val_e: (to_val e) => [v|].
-  { iExists v, [], σ, ns, ks, nt. iMod "IH". iFrame.
-    rewrite app_nil_r -(of_to_val _ _ val_e). eauto. }
+  { iExists v, σ, ns, ks, nt. iMod "IH". iFrame.
+    rewrite -(of_to_val _ _ val_e). by eauto. }
   iMod ("IH" with "state") as (red_e) "IH".
   case: red_e => e' [] σ' [] es' Hstep.
   iMod ("IH" with "[//]") as "(_ & state & [IH _] & _)".
   iSpecialize ("IH" with "[//]").
-  iMod ("IH" $! es1 (es2 ++ es') with "state")
-    as (v es'' σ'' ns' ks' nt' Hexec) "state".
-  have {}Hstep : erased_step (es1 ++ e :: es2, σ) (es1 ++ e' :: es2 ++ es', σ').
-  { exists []. econstructor; eauto. }
-  iModIntro. iExists v, (es' ++ es''), σ'', ns', ks', nt'. iFrame.
-  iPureIntro. rewrite -app_assoc in Hexec. by eapply rtc_l; eauto.
+  iMod ("IH" with "state") as (v σ'' ns' ks' nt' Hexec) "state".
+  have {}Hstep : thread_step (e, σ) (e', σ').
+  { by exists es' => /=. }
+  iModIntro. iExists v, σ'', ns', ks', nt'. iFrame.
+  iPureIntro. by eapply rtc_l; eauto.
 Qed.
 End adequacy.
 
-Theorem twp_rtc Σ Λ `{!invGpreS Σ} e es1 es2 σ P n :
+Theorem twp_rtc Σ Λ `{!invGpreS Σ} e σ P n :
   (∀ `{Hinv : !invGS_gen HasNoLc Σ},
      ⊢ |={⊤}=> ∃
          (stateI : state Λ → nat → list (observation Λ) → nat → iProp Σ)
@@ -60,15 +60,13 @@ Theorem twp_rtc Σ Λ `{!invGpreS Σ} e es1 es2 σ P n :
            IrisG Hinv stateI fork_post num_laters_per_step state_interp_mono
        in
        stateI σ n [] 0 ∗ WP e [{ v, ⌜ P v ⌝ }]) →
-  ∃ v es' σ',
-  rtc erased_step (es1 ++ e :: es2, σ) (es1 ++ of_val v :: es2 ++ es', σ') ∧
-  P v.
+  ∃ v σ', rtc thread_step (e, σ) (of_val v, σ') ∧ P v.
 Proof.
   intros Hwp. eapply pure_soundness.
   apply (fupd_soundness_no_lc ⊤ ⊤ _ 0)=> Hinv. iIntros "_".
   iMod (Hwp) as (stateI num_laters_per_step fork_post stateI_mono) "[Hσ H]".
   set (iG := IrisG Hinv stateI fork_post num_laters_per_step stateI_mono).
   iPoseProof (twp_runs_until with "H") as "H".
-  iMod ("H" $! es1 es2 with "Hσ") as (v es' σ' ns' ks' nt' Hexec) "[_ %post]".
+  iMod ("H" with "Hσ") as (v σ' ns' ks' nt' Hexec) "[_ %post]".
   iModIntro. iPureIntro. by eauto.
 Qed.
