cryptis/lib/adequacy.v
@@ -4,13 +4,12 @@ From iris.program_logic Require Export total_adequacy.
 From iris.heap_lang Require Export adequacy.
 From iris.heap_lang Require Import proofmode notation.
 From iris.prelude Require Import options.
+From cryptis Require Import lib.
 From cryptis.lib Require Import gen_adequacy.
 
-Lemma heap_twp_rtc Σ `{!heapGpreS Σ} e es1 es2 σ φ :
+Lemma heap_twp_thread_exec Σ `{!heapGpreS Σ} e σ φ :
   (∀ `{!heapGS_gen HasNoLc Σ}, ⊢ inv_heap_inv -∗ WP e [{ v, ⌜φ v⌝ }]) →
-  ∃ v es' σ',
-  rtc erased_step (es1 ++ e :: es2, σ) (es1 ++ of_val v :: es2 ++ es', σ') ∧
-  φ v.
+  ∃ v σ', rtc thread_step (e, σ) (of_val v, σ') ∧ φ v.
 Proof.
   intros Hwp; eapply (twp_rtc _ _); iIntros (?) "".
   iMod (gen_heap_init σ.(heap)) as (?) "[Hh _]".
@@ -24,4 +23,28 @@ Proof.
                    mono_nat_auth_own γ 1 ns)%I),
     id, (λ _, True%I), _; iFrame.
   by iApply (Hwp (HeapGS _ _ _ _ _ _ _ _)).
+Qed.
+
+Lemma thread_exec_pure_exec (e : expr) σ e' σ' :
+  rtc thread_step (e, σ) (e', σ') →
+  pure_expr e →
+  rtc pure_step e e'.
+Proof.
+set t := (e, σ); set t' := (e', σ').
+rewrite -[e]/(t.1) -[e']/(t'.1); move: t t' => t t' {e σ e' σ'}.
+elim: t t' / => //= - [e σ] [e' σ'] [e'' σ''] [/= efs Hstep] _ IH pure_e.
+have pure_e' : pure_expr e' by apply: pure_exprP.
+have {}Hstep : pure_step e e' by apply: pure_expr_pure_step.
+by apply: rtc_l; eauto.
+Qed.
+
+Lemma heap_twp_pure_exec Σ `{!heapGpreS Σ} e φ :
+  pure_expr e →
+  (∀ `{!heapGS_gen HasNoLc Σ}, ⊢ inv_heap_inv -∗ WP e [{ v, ⌜φ v⌝ }]) →
+  ∃ v, rtc pure_step e (of_val v) ∧ φ v.
+Proof.
+move=> pure_e /heap_twp_thread_exec Hwp.
+have [v [] σ' [] Hexec post] := Hwp {| heap := ∅; used_proph_id := ∅ |}.
+exists v; split => //.
+exact: thread_exec_pure_exec Hexec pure_e.
 Qed.
